Implementation of lgen function done. Now need to prove its properties.

LeastGen.v
@@ -1,10 +1,117 @@
 Set Implicit Arguments.
 
-Require Import OrderedTypeEx Arith_base.
+Require Import Recdef List.
+
 Require Import LibTactics.
-Require Import FMapInterface.
-Require Import FMapAVL.
-Require Import FMapFacts.
+Require Import TyOrder Subst Ty Monad Arith_base.
+
+Include SUBST.
+Include TYORDER.
+
+Fixpoint lgen_aux (t t' : ty) : M ty :=
+  match t,t' with
+    | tvar n, tvar n' => 
+      _ <- freshVar ;
+      _ <- freshVar ;
+      lookup_gen (tvar n) (tvar n')
+    | tvar n, tcon n' =>
+      _ <- freshVar ;
+      lookup_gen (tvar n) (tcon n')
+    | tvar n, tapp l r =>
+      _ <- freshVar ;
+      lookup_gen (tvar n) (tapp l r)
+    | tcon n, tvar n' =>
+      _ <- freshVar ;
+      lookup_gen (tcon n) (tvar n')
+    | tcon n, tcon n' =>
+      if eq_nat_dec n n' then 
+        ret (tcon n) 
+        else 
+          lookup_gen (tcon n) (tcon n')
+    | tcon n, tapp l r =>
+      lookup_gen (tcon n) (tapp l r)
+    | tapp l r, tvar n =>
+      _ <- freshVar  ;
+      lookup_gen (tapp l r) (tvar n)
+    | tapp l r, tcon n =>
+      lookup_gen (tapp l r) (tcon n)
+    | tapp l r, tapp l' r' =>
+      lg <- lgen_aux l l' ;
+      rg <- lgen_aux r r' ;
+      ret (tapp lg rg)
+  end.
+
+Definition lgen (t t' : ty) : ty :=
+  snd (lgen_aux t t' (mkState 0 nil)).
+
+Section LGEN_Properties.
+ Ltac my_simpl := 
+   repeat (
+     match goal with
+       | [H : (tcon _) <=: (tvar _) |- _] => destruct H as [x Hx] ; inverts Hx
+       | [H : (tapp _ _) <=: (tvar _) |- _] => destruct H as [x Hx] ; inverts Hx
+       | [H : (tapp _ _) <=: (tcon _) |- _] => destruct H as [x Hx] ; inverts Hx
+       | [H : (tcon _) <=: (tapp _ _) |- _] => destruct H as [x Hx] ; inverts Hx
+       | [|- exists _, TyOrder.apply_subst_on_ty _ (tvar ?n) = ?s] => 
+         exists (M.add n s (@M.empty ty)) ; simpl ; rewrite add_o ; case_if*
+     end).
+  
+  (** first property: generalization **)
+
+  Theorem lgen_is_gen : forall t t' s, lgen t t' = s -> s <=: t /\ s <=: t'.
+  Proof.
+    intros t ; induction t ; intros t' s H ; split ; 
+      cases* t' as Ht ; inverts H ; unfolds ; unfold lgen ; simpl.
+
+    exists (M.add 2 (tvar n) (@M.empty ty)). rewrite add_o. case_if*.
+     
+    exists (M.add 1 (tvar n) (@M.empty ty)). rewrite add_o. case_if*.
+
+    exists (M.add 1 (tvar n) (@M.empty ty)). rewrite add_o. case_if*.
+
+    exists (M.add 2 (tvar n0) (@M.empty ty)). rewrite add_o. case_if*.
+    
+    exists (M.add 1 (tcon n0) (@M.empty ty)). rewrite add_o. case_if*.
+
+    exists (M.add 1 (tapp TEMP1 TEMP2) (@M.empty ty)). rewrite add_o. case_if*.
+
+    exists (M.add 1 (tcon n) (@M.empty ty)). rewrite add_o. case_if*.
+
+    exists (M.add 0 (tcon n) (@M.empty ty)). case_if*.
+
+    exists (M.add 0 (tcon n) (@M.empty ty)). rewrite add_o. case_if*.
+
+    exists (M.add 1 (tvar n0) (@M.empty ty)). rewrite add_o. case_if*.
+
+    case_if*. exists (@M.empty ty). simpl. auto.
+
+    simpl. exists (M.add 0 (tcon n0) (@M.empty ty)). rewrite add_o. case_if*.
+    
+    exists (M.add 0 (tapp TEMP1 TEMP2) (@M.empty ty)). rewrite add_o. case_if*.
+
+    exists (M.add 1 (tapp t1 t2) (@M.empty ty)). rewrite add_o. case_if*.
+
+    exists (M.add 0 (tapp t1 t2) (@M.empty ty)). rewrite add_o. case_if*.
+
+    admit.
+
+    exists (M.add 1 (tvar n) (@M.empty ty)). rewrite add_o. case_if*.
+    
+    exists (M.add 0 (tcon n) (@M.empty ty)). rewrite add_o. case_if*.
+
+    admit.
+  Qed. 
+
+  Theorem lgen_is_least : forall t t' s, lgen t t' = s -> forall u, u <=: t /\ u <=: t' -> u <=: s.
+  Proof.
+    intro t ; induction t ; intros t' s H ; destruct t' ; intros u [Hu1 Hu2] ; destruct* u ; unfolds ; try my_simpl.
+
+    destruct Hu1 as [s1 Hu1]. destruct Hu2 as [s2 Hu2]. simpl in Hu1, Hu2.
+    rewrite <- Hu1 in H. rewrite Hu2 in H. unfolds in H. simpl in H. cases_if*.
+    simpl in H. subst. rewrite Hu2. exists (@M.empty ty). auto.
+
+  Qed.
+End LGEN_Properties.
 
 
 
