TyOrder.v
@@ -23,4 +23,44 @@ Module TYORDER.
       rewrite compose_apply.
       rewrite* <- H1 in H2.
     Qed.
+
+    (** Definition of alpha-equivalence between types **)
+
+    Definition renaming_subst (s : subst) := forall n t, M.find n s = Some t -> exists v, t = tvar v.
+
+    Remark null_subst_is_renaming : renaming_subst (@M.empty ty).
+    Proof.
+      unfolds ; introv H.
+      rewrite empty_o in H. congruence.
+    Qed.
+
+    Remark compose_renaming : forall (s1 s2 : subst), renaming_subst s1 -> renaming_subst s2 -> renaming_subst (s1 @@ s2).
+    Proof.
+      introv H1 H2 ; unfold renaming_subst in * ; introv H3.
+      admit.
+    Qed.
+
+    Inductive alpha_eq : ty -> ty -> Prop :=
+      | ae_var : forall n n', alpha_eq (tvar n) (tvar n')
+      | ae_con : forall n n', n = n' -> alpha_eq (tcon n) (tcon n')
+      | ae_app : forall t1 t2 t1' t2',  alpha_eq t1 t1' ->
+                                        alpha_eq t2 t2' ->
+                                        alpha_eq (tapp t1 t2) (tapp t1' t2').
+
+    Theorem alpha_eq_is_renaming : 
+      forall t t', alpha_eq t t' <-> exists s, renaming_subst s /\ apply_subst_on_ty s t = t'.
+    Proof.
+      intros t t' ; split ; intros H ; [induction H | idtac].
+        exists (M.add n (tvar n') (@M.empty ty)) ; split.
+          unfolds. introv H. rewrite add_o in H.
+          cases_if in H. inverts* H. 
+          rewrite empty_o in H. congruence.
+          simpl. rewrite add_o. cases_if*.         
+        subst. exists (@M.empty ty) ; split ; [apply null_subst_is_renaming | auto].
+        destruct IHalpha_eq1 as [s1 [Hr1 Ha1]].
+        destruct IHalpha_eq2 as [s2 [Hr2 Ha2]].
+        exists (s2 @@ s1) ; split. applys* compose_renaming. rewrite compose_apply ; auto.
+        simpl. admit.
+      admit.
+    Qed.
 End TYORDER.
