Monad.v
@@ -1,0 +1,57 @@
+(** Simple state monad for use in the 
+    least generalization function **)
+
+Set Implicit Arguments.
+
+Require Import List Ty.
+
+(** Representation of the state **)
+
+Record state := mkState {
+  st_next_tvar : nat ;               (** fresh variable generalization **)
+  st_list_gen  : list (ty * ty * ty) (** list of generalizations done by the algorithm **)
+}.
+
+(** Concrete monad type definition **)
+
+Definition M (A : Type) := state -> (state * A).
+
+Definition ret (A : Type)(x : A) : M A := fun s => (s,x).
+
+Definition bind(A B : Type)(c1 : M A)(c2: A -> M B) : M B :=
+  fun s1 =>
+    match c1 s1 with
+      |(s2,v) => c2 v s2
+    end.
+
+Notation "x <- c1 ; c2" := (bind c1 (fun x => c2))
+  (right associativity, at level 84, c1 at next level).
+
+Definition freshVar : M nat :=
+  fun s =>
+    match s with
+      | mkState n m => (mkState (S n) m, n)
+    end.
+
+Fixpoint lookup_gen_aux (t t' : ty) (m : list (ty * ty * ty)) : option ty :=
+  match m with
+    | nil => None
+    | (t1,t2,t3) :: m' =>
+      match eq_ty_dec t t1, eq_ty_dec t' t2 with
+        | left _, left _ => Some t3
+        | left _, right _ => None
+        | right _, left _ => None
+        | right _, right _ => None
+      end
+  end.
+
+Definition lookup_gen (t t' : ty) : M ty :=
+  fun s =>
+    match s with
+      | mkState n m =>
+        match lookup_gen_aux t t' m with
+          | None => 
+            (mkState (S n) ((t,t',(tvar n)) :: m), tvar n)
+          | Some t => (s,t)
+        end
+    end.
