Ty.v
@@ -5,9 +5,19 @@ Inductive ty : Set :=
   | tcon : nat -> ty
   | tapp : ty -> ty -> ty.
 
+Fixpoint ty_size (t : ty) : nat :=
+  match t with
+    | tvar _ => 0
+    | tcon _ => 1
+    | tapp l r => 1 + (ty_size l) + (ty_size r)
+  end.
+
+Definition ty_pair_size (t t' : ty) : nat :=
+  (ty_size t) + (ty_size t').
+
 (** equality on types is decidable **)
 
-Definition eq_type_dec : forall (t t' : ty), {t = t'} + {t <> t'}.
+Definition eq_ty_dec : forall (t t' : ty), {t = t'} + {t <> t'}.
    pose eq_nat_dec.
    decide equality.
 Defined.
